NewExamples.v
@@ -1,0 +1,552 @@
+Require Import Crypto.
+Require Import ProtoRep.
+Require Import ProtoSemantics.
+Require Import CpdtTactics.
+Require Import Arith.
+
+(* Simple increment example *)
+
+Definition incPayload (m:message Basic) : (message Basic) :=
+  match m with
+  | basic n => basic (n + 1)
+  | _ => bad Basic                 
+  end.
+
+Definition proto1A (m:(message Basic)) :=
+  send m;
+  x <- receive;
+  ReturnC (t:=Basic) x.
+Check proto1A.
+
+Definition proto1B :=
+  x <- receive;
+  send (incPayload x);
+  ReturnC x.
+Check proto1B.
+
+Theorem dual1AB : forall (x:message Basic), Dual (proto1A x) proto1B.
+Proof.
+  cbv.
+  split.
+  reflexivity.
+  split.
+    reflexivity.
+    trivial.
+Qed.
+
+Theorem incPropertyAB : forall x x' st st',
+    multi st _ _ _ (proto1A x) proto1B (ReturnC x') st' ->
+    x' = incPayload x.
+Proof.
+  intros x x' st st' multiProof.
+  dep_destruct multiProof. clear multiProof.
+  dep_destruct s0. dep_destruct s1. clear s0. clear s1.
+  dep_destruct x2. clear x2.
+  dep_destruct s0. dep_destruct s1. clear s0. clear s1.
+  dep_destruct x3. reflexivity.
+  inversion s1.
+Qed.
+
+
+(* Needham Schroeder *)
+
+Definition Nonce := Basic.
+Definition Id := Basic.
+Definition null := basic 0.
+
+Definition resT := Pair (Pair Nonce Nonce) Id.
+Definition res : message resT :=
+  pair _ _ (pair _ _ (bad Nonce) (bad Nonce)) (bad Id).
+Print res.
+Definition ares : message resT :=
+  pair _ _ (pair _ _ (basic 0) (bad Nonce)) (bad Id).
+Print ares.
+Definition bres : message resT :=
+  pair _ _ (pair _ _ (bad Nonce) (basic 0)) (bad Id).
+Print bres.
+Definition idres : message resT :=
+  pair _ _ (pair _ _ (bad Nonce) (bad Nonce)) (basic 0).
+Print idres.
+
+Definition getAnonce (rIn:message resT) : message Nonce :=
+  pairFst (pairFst rIn).
+Eval compute in getAnonce ares.
+Eval compute in getAnonce bres.
+Eval compute in getAnonce idres.
+
+Definition getBnonce (rIn:message resT) : message Nonce :=
+  pairSnd (pairFst rIn).
+Eval compute in getBnonce ares.
+Eval compute in getBnonce bres.
+Eval compute in getBnonce idres.
+
+Definition getId (rIn:message resT) : message Id :=
+  pairSnd rIn.
+
+Eval compute in getId ares.
+Eval compute in getId bres.
+Eval compute in getId idres.
+
+Definition updateA (aNonce:message Nonce) (rIn:message resT) : message resT :=
+  pair _ _ (pair _ _ aNonce (getBnonce rIn)) (getId rIn).
+
+Eval compute in updateA (basic 0) res.
+
+Definition updateB (bNonce:message Nonce) (rIn:message resT) : message resT :=
+  pair _ _ (pair _ _ (getAnonce rIn) bNonce) (getId rIn).
+
+Eval compute in updateB (basic 0) res.
+
+Definition updateId (id:message Id) (rIn:message resT) : message resT :=
+  pair _ _ (pair _ _ (getAnonce rIn) (getBnonce rIn)) id.
+
+Eval compute in updateId (basic 0) res.
+
+Definition initT := Pair Nonce Id.
+Definition init : message initT
+  := pair _ _ (bad Nonce) (bad Id).
+
+Definition getPubkey (m:message Id) :=
+  match m with
+  | basic n => public n
+  | _ => public 0
+  end.
+
+Definition bLast (id:message Id) (aRes:message resT) :=
+  x <- receive;
+  ReturnC (pair Nonce _ x id).
+
+Definition iLast :=
+  x <- receive;
+  send x;
+  ReturnC (t:=Encrypt Nonce) x.
+
+Definition aLast (id:message Id) (aRes:message resT) :=
+  x <- receive;
+  let na := pairFst (t1:=Nonce) x in
+  let nb := pairSnd x in
+      send (encrypt Nonce nb (getPubkey id));
+    ReturnC null.
+
+Definition extractPayload (m:message Basic) : nat :=
+  match m with
+  | basic n => n
+  | _ => 0
+  end.
+
+Definition aId : (message Id) := (basic 0).
+Definition bId : (message Id) := (basic 1).
+Definition iId : (message Id) := (basic 2).
+
+Definition nslA (myPri:keyType) (theirId:message Id) :=
+  let myNonce := basic 0 in
+  let myId        : (message Id)    := aId  in
+  let theirPubkey : (keyType)       := (getPubkey theirId) in 
+  let s1          : (message (Encrypt (Pair Nonce Id)))
+                                    := encrypt _
+                                       (pair _ _ myNonce myId) theirPubkey in
+  send s1;
+  r1 <- receive;
+  let decTry      : (message (Pair (Pair Nonce Nonce) Id))
+                                    := decryptM r1 myPri in
+  let myNonce'    : (message  Nonce)
+                                    := pairFst (pairFst decTry) in
+  let theirNonce  : (message Nonce) := pairSnd (pairFst decTry) in
+  let newId       : (message Id)    := pairSnd decTry in
+  let newPubkey   : (keyType)       := (getPubkey newId) in
+  let s2          : (message (Encrypt Nonce))
+                                    := encrypt _ theirNonce newPubkey in
+  send s2;
+  ReturnC (pair _ _ myNonce' theirNonce).
+Check nslA.
+
+Definition nslB (myPri:keyType) (intruder:bool) :=
+  r1 <- receive;
+  let myId        : (message Id)    := bId  in
+  let myNonce     : (message Nonce) := (basic 1) in
+  let newR1       : (message (Encrypt(Pair Nonce Id)))
+                    := if (intruder) then
+                         let decI := decryptM r1 (private 2) in
+                           encrypt _ decI (getPubkey bId)
+                       else
+                         r1 in
+  let decB := decryptM newR1 myPri in
+  let they := extractPayload (pairSnd decB) in
+  let theirNonce := pairFst decB in
+  let theirId := pairSnd decB in
+  let theirPub := (public they) in
+  let s1 := encrypt _
+             (pair _ _ (pair _ _ theirNonce myNonce) myId) (theirPub) in
+  send s1;
+  r2 <- receive;
+  let decB2 := if (intruder) then
+                 decryptM r2 (private 2)
+               else decryptM r2 myPri in
+  let myNonce' := decB2 in
+  let ab := pair Nonce Nonce theirNonce myNonce' in
+  ReturnC (pair _ _ ab theirId).
+Check nslB.
+
+Example dualab : forall x y z b, Dual (nslA x y) (nslB z b).
+Proof.
+  intros; unfold nslA; unfold nslB; cbn;
+  split. reflexivity.
+  split. reflexivity.
+  split. reflexivity.
+  trivial.
+Defined.
+
+Definition expectedA :=
+  pair _ _ (basic 0) (basic 1).
+
+Definition expectedB :=
+  pair _ _
+       (pair _ _ (basic 0) (basic 1))
+       aId.
+
+
+Example aResult :
+  let intruder := false in
+  let theirId := if(intruder)
+                 then iId
+                 else bId in
+  let aPri := (private 0) in
+  let bPri := (private 1) in
+  
+  forall st m, 
+    multi st _ _ _ (nslA aPri theirId) (nslB bPri intruder) (ReturnC m) st ->
+    (m = expectedA).
+Proof.
+  intros.
+  unfold nslA. unfold nslB.
+  dep_destruct H. clear H.
+  dep_destruct s0. dep_destruct s1. clear s0. clear s1.
+  dep_destruct x1. clear x1. dep_destruct s0. dep_destruct s1. clear s0. clear s1.
+  dep_destruct x2. clear x2. dep_destruct s0. dep_destruct s1. clear s0. clear s1.
+  dep_destruct x1. clear x1. reflexivity.
+  inversion s1.
+Qed.
+
+Example bResult :
+  let intruder := false in
+  let theirId := if(intruder)
+                 then iId
+                 else bId in
+  let aPri := (private 0) in
+  let bPri := (private 1) in
+  
+  forall st m, 
+    multi st _ _ _ (nslB bPri intruder) (nslA aPri theirId) (ReturnC m) st ->
+    (m = expectedB).
+Proof.
+  intros.
+  unfold nslA. unfold nslB.
+  dep_destruct H. clear H.
+  dep_destruct s0. dep_destruct s1. clear s0. clear s1.
+  dep_destruct x1. clear x1. dep_destruct s0. dep_destruct s1. clear s0. clear s1.
+  dep_destruct x2. clear x2. dep_destruct s1. dep_destruct s3. clear s1. clear s3.
+  dep_destruct x1. clear x1. cbv. reflexivity.
+  inversion s3.
+Qed.
+
+Definition nsA (myPri:keyType) (theirId:message Id) :=
+  let myNonce := basic 0 in
+  let myId        : (message Id)    := aId  in
+  let theirPubkey : (keyType)       := (getPubkey theirId) in 
+  let s1          : (message (Encrypt (Pair Nonce Id)))
+                                    := encrypt _
+                                       (pair _ _ myNonce myId) theirPubkey in
+  send s1;
+  r1 <- receive;
+  let decTry      : (message (Pair Nonce Nonce))
+                                    := decryptM r1 myPri in
+  let myNonce'    : (message  Nonce)
+                                    := (pairFst decTry) in
+  let theirNonce  : (message Nonce) := (pairSnd decTry) in
+  (*let newId       : (message Id)    := pairSnd decTry in*)
+  let newPubkey   : (keyType)       := (getPubkey theirId(*newId*)) in
+  let s2          : (message (Encrypt Nonce))
+                                    := encrypt _ theirNonce newPubkey in
+  send s2;
+  ReturnC (pair _ _ myNonce' theirNonce).
+Check nsA.
+
+Definition nsB (myPri:keyType) (intruder:bool) :=
+  r1 <- receive;
+  (*let myId        : (message Id)    := bId  in*)
+  let myNonce     : (message Nonce) := (basic 1) in
+  let newR1       : (message (Encrypt(Pair Nonce Id)))
+                    := if (intruder) then
+                         let decI := decryptM r1 (private 2) in
+                           encrypt _ decI (getPubkey bId)
+                       else
+                         r1 in
+  let decB := decryptM newR1 myPri in
+  let they := extractPayload (pairSnd decB) in
+  let theirNonce := pairFst decB in
+  let theirId := pairSnd decB in
+  let theirPub := (public they) in
+  let s1 := encrypt _
+             (pair _ _ theirNonce myNonce) (theirPub) in
+  send s1;
+  r2 <- receive;
+  let decB2 := if (intruder) then
+                 decryptM r2 (private 2)
+               else decryptM r2 myPri in
+  let myNonce' := decB2 in
+  let ab := pair Nonce Nonce theirNonce myNonce' in
+  ReturnC (pair _ _ ab theirId).
+Check nsB.
+
+Example dualab' : forall x y z b, Dual (nsA x y) (nsB z b).
+Proof.
+  intros; unfold aa; unfold bb; cbn;
+  split. reflexivity.
+  split. reflexivity.
+  split. reflexivity.
+  trivial.
+Defined.
+
+
+Example bResult' :
+  let intruder := true in
+  let theirId := if(intruder)
+                 then iId
+                 else bId in
+  let aPri := (private 0) in
+  let bPri := (private 1) in
+  
+  forall st m, 
+    multi st _ _ _ (nsB bPri intruder) (nsA aPri theirId) (ReturnC m) st ->
+    (m = expectedB).
+Proof.
+  intros.
+  unfold aa. unfold bb.
+  dep_destruct H. clear H.
+  dep_destruct s0. dep_destruct s1. clear s0. clear s1.
+  dep_destruct x1. clear x1. dep_destruct s0. dep_destruct s1. clear s0. clear s1.
+  dep_destruct x2. clear x2. dep_destruct s1. dep_destruct s3. clear s1. clear s3.
+  dep_destruct x1. clear x1. cbv. simpl. reflexivity.
+  inversion s3.
+Qed.
+  
+    
+
+
+
+
+
+
+
+
+
+
+
+
+
+
+
+
+
+
+
+
+
+Definition aNonceSecret := 11.
+Definition bNonceSecret := 22.
+Definition aNonce := (basic aNonceSecret).
+Definition bNonce := (basic bNonceSecret).
+
+Definition aPub := (public 1).
+Definition bPub := (public 2).
+Definition aPubBad := (public 3).
+Definition bPubBad := (public 4).
+Definition aPri := (private 1).
+Definition bPri := (private 2).
+Definition aPriBad := (private 5).
+Definition bPriBad := (private 6).
+
+Definition oneEnc := (encrypt _ (basic 0) (public 0)).
+Definition twoEnc := (encrypt _ oneEnc (public 1)).
+
+Eval compute in oneEnc.
+Eval compute in twoEnc.
+
+Definition oneDec := decryptM twoEnc (private 2).
+Eval compute in oneDec.
+
+Definition twoDec := decryptM oneDec (private 0).
+Eval compute in twoDec.
+
+Eval compute in decryptM (bad (Encrypt Basic)) (public 0).
+
+Definition Needham_A (myPri theirPub:keyType) :=
+  send (encrypt _ aNonce theirPub);
+  x <- receive; (* x : Encrypt (Pair Basic Basic) *) 
+  let y : (message (Pair Basic Basic)):= decryptM x myPri in (* y : Pair Basic Basic *)
+  let y' := (pairFst y) in
+  let y'' := (pairSnd y) in 
+  send (encrypt _ y'' theirPub);
+  ReturnC (pair _ _ y' y''). Check Needham_A.
+
+Definition Needham_B (myPri theirPub:keyType) :=
+  ReceiveC (fun x: message (Encrypt Basic) => ( 
+  (*x <- receive; (* x : Encrypt Basic *) *)
+  let y : (message Basic) := decryptM x myPri in (* y : Basic *)
+  send (encrypt (Pair Basic Basic) (pair _ _ y bNonce) theirPub);
+  ReceiveC (fun z : message (Encrypt Basic) => ( 
+  (*z <- receive; (* z : Encrypt Basic *) *)
+                let z' := decryptM z myPri in   (* z' : Basic *)
+  (*ReturnC y)))).  Check Needham_B. *)
+  ReturnC (pair _ _ y z'))))). Check Needham_B.
+
+Example dualNeedham : forall ka ka' kb kb',
+    Dual (Needham_A ka kb') (Needham_B kb ka').
+Proof.
+  intros.
+  split. reflexivity.
+  split. reflexivity.
+  split. reflexivity.
+  reflexivity.
+Qed.
+
+(*
+
+Theorem needham_A_auth : forall (k:keyType) (x:message Basic) st st', 
+    multi
+      st
+      _ _ _
+      (Needham_A k bPub)
+      (Needham_B bPri aPub)
+      (ReturnC (pair _ _ x bNonce))
+      st'
+    -> (k = inverse aPub).
+Proof.
+  intros k x st st' multiProof.
+  dep_destruct multiProof. clear multiProof.
+  dep_destruct s0. dep_destruct s1. clear s0. clear s1.
+  dep_destruct x2. clear x2.
+  dep_destruct s0. dep_destruct s1. clear s0. clear s1.
+  dep_destruct x3. clear x3.
+  dep_destruct s1. dep_destruct s4. clear s1. clear s4.
+  dep_destruct x2. clear x2. clear x. cbn in x0.
+  unfold decryptM in x0.
+  destruct  (decrypt
+            (encrypt _ (pair _ _ aNonce (basic bNonceSecret)) aPub)
+            k) as [p | _].
+  destruct p as (m , i).
+    dep_destruct i. reflexivity. simpl in x0.
+    inversion x0.
+  inversion s4.
+Qed.
+
+
+Definition normalizeState : State -> State := fun _ => emptyState.
+
+(* Future Work *)
+Definition hoare_triple{p1t p2t p3t:protoType}{t:type}
+           (P:Assertion)
+           (p1:protoExp p1t) (p2:protoExp p2t) (p3:protoExp p3t)
+           (Q:Assertion) : Prop :=
+  forall st st',
+     P st ->
+     multi st _ _ _ p1 p2 p3 st' ->
+     Q (normalizeState st').
+
+Definition notInPb : (message Basic) -> State -> Prop := fun _ _ => True.
+Definition inPb : (message Basic) -> State -> Prop := fun _ _ => True.
+
+
+Definition learnedB {p1t p2t p3t:protoType}
+           (m:message Basic)
+           (p1:protoExp p1t) (p2:protoExp p2t) (p3:protoExp p3t) : Prop :=
+  hoare_triple (t:=Basic) (notInPb m) p1 p2 p3 (inPb m).
+ 
+
+Definition p1 :=
+  send (basic 33);
+  EpsC.
+
+Definition p2 :=
+  x <- receive;
+  ReturnC (t:=Basic) x.
+
+Definition learnedProof : learnedB (basic 33) p2 p1 (ReturnC (basic 33)).
+Proof.
+  intros.
+  unfold p1. unfold p2. unfold learnedB. unfold hoare_triple.
+  intros.
+  dep_destruct H0. clear H0.
+  dep_destruct s0. dep_destruct s1. clear s0. clear s1.
+  dep_destruct x1. clear x1. simpl. cbn. trivial.
+  Abort.
+
+
+
+
+
+
+
+
+(* Simplest possible encrypt/decrypt protocol pair *)
+Definition protoEncrypt1 (theirPub:keyType) :=
+  send (encrypt _ (basic 42) theirPub);
+  EpsC.
+
+Definition protoDecrypt1 (myPri:keyType) :=
+  x <- receive;
+  ReturnC (t:=Basic) (decryptM x myPri).
+
+Example result1 : 
+    multi
+      emptyState
+      _ _ _
+      (protoDecrypt1 (private 1))
+      (protoEncrypt1 (public 1))
+      (ReturnC (basic 42))
+      (updateState (encrypt Basic (basic 42) (public 1)) emptyState).
+Proof.
+  eapply multi_step with (st2:=emptyState).
+  constructor.
+  constructor.
+  apply multi_refl.
+Qed.
+
+Example auth1 : forall k k',
+    multi
+      emptyState
+      _ _ _
+      (protoDecrypt1 k')
+      (protoEncrypt1 k)
+      (ReturnC (basic 42))
+      (updateState (encrypt Basic (basic 42) (public 1)) emptyState)
+      -> (k = inverse k').
+Proof.
+  intros.
+  dep_destruct H. dep_destruct s0. dep_destruct x1.
+  apply decryptSuccess with (m:= (basic 42)).
+  unfold not. intros. inversion H0.
+  assumption.
+  dep_destruct s2.
+Qed.
+
+Example auth1' : forall k k' st',
+    multi
+      emptyState
+      _ _ _
+      (protoDecrypt1 k')
+      (protoEncrypt1 k)
+      (ReturnC (basic 42))
+      st'
+      -> (k = inverse k').
+Proof.
+  intros.
+  dep_destruct H. clear H. dep_destruct s0. clear s0. dep_destruct x1.
+  apply decryptSuccess with (m:= (basic 42)).
+  unfold not. intros. inversion H.
+  assumption.
+  inversion s2.
+Qed.
+*)
+
+
