State.v
@@ -1,0 +1,99 @@
+Require Import Crypto.
+Require Import SfLib.
+
+Definition ob (t:type) := list ((message t) * (list (message Key))).
+
+Record State : Type := mkState
+        {keys : list (message Key);
+         basics : list (message Basic);
+         kOb : ob Key;
+         bOb : ob Basic 
+        }.
+
+Definition emptyState := mkState nil nil nil nil.
+
+Definition Assertion := State -> Prop.
+
+Definition addKey : forall mt (m:message mt) (pf: mt = Key),
+    (list (message Key)) -> (list (message Key)).
+Proof.
+  intros. subst. exact (m :: X).
+Defined.
+
+Definition addMKey t (m:message t) : (list (message Key)) -> (list (message Key)) := fun l => (
+  match t as t' return (t = t') -> (list (message Key)) with
+  | Key => fun pf => (addKey t m pf l)
+  | _ => fun _ => l
+  end (eq_refl t)).
+
+Definition addBasic : forall mt (m:message mt) (pf: mt = Basic),
+    (list (message Basic)) -> (list (message Basic)).
+Proof.
+  intros. subst. exact (m :: X).
+Defined.
+
+Definition addMBasic t (m:message t) : (list (message Basic)) -> (list (message Basic)) := fun l => (
+  match t as t' return (t = t') -> (list (message Basic)) with
+  | Basic => fun pf => (addBasic t m pf l)
+  | _ => fun _ => l
+  end (eq_refl t)).
+
+Definition addP (t:type) : forall mt (pf:mt = t),  ((message mt) * (list (message Key))) -> (ob t) -> (ob t).
+Proof.
+  intros. subst. exact (X :: X0 ).
+Defined.
+
+Definition addMp mt (p:((message mt)*(list (message Key)))) : (ob Basic) -> (ob Basic) := fun l => (
+  match mt as t' return (mt = t') -> (ob Basic) with
+  | Basic => fun pf => (addP _ _ pf p l)
+  | _ => fun _ => l
+  end (eq_refl mt)).
+
+Definition addMpK mt (p:((message mt)*(list (message Key)))) : (ob Key) -> (ob Key) := fun l => (
+  match mt as t' return (mt = t') -> (ob Key) with
+  | Key => fun pf => (addP _ _ pf p l)
+  | _ => fun _ => l
+  end (eq_refl mt)).
+
+Fixpoint obligations'{mt:type} (m:message mt) (kl: list (message Key))
+                               (l:ob Basic) : ob Basic :=
+  match m with
+  | encrypt mt' m' k => match mt' with
+                       | Basic => let new := (m', (kl ++ [(key k)])) in
+                                 addMp mt' new l
+                       | _ => obligations' m' (kl ++ [(key k)]) l
+                       end
+  | pair _ _ m1 m2 => (obligations' m1 kl l) ++ (obligations' m2 kl l)
+  | basic n => addMp _ ((basic n), kl) l
+  | _ => addMp _ (m, nil) l                                           
+  end.
+
+
+Definition obligations{mt:type} (m:message mt) : ob Basic :=
+  obligations' m nil nil.
+
+Fixpoint obligationsK'{mt:type} (m:message mt) (kl: list (message Key))
+                               (l:ob Key) : ob Key :=
+  match m with
+  | encrypt mt' m' k => match mt' with
+                       | Key => let new := (m', (kl ++ [(key k)])) in
+                                 addMpK _ new l
+                       | _ => obligationsK' m' (kl ++ [(key k)]) l
+                       end
+  | pair _ _ m1 m2 => (obligationsK' m1 kl l) ++ (obligationsK' m2 kl l)
+  | key k => addMpK _ ((key k), kl) l 
+  | _ => addMpK _ (m, nil) l                                           
+  end.
+
+Definition obligationsK{mt:type} (m:message mt) : ob Key :=
+  obligationsK' m nil nil.
+
+Definition updateState{t:type} (m:message t) (sIn: State) : State :=
+  match t with
+  | Basic => mkState  sIn.(keys) (addMBasic t m sIn.(basics)) sIn.(kOb) sIn.(bOb)
+  | Key => mkState (addMKey t m sIn.(keys)) sIn.(basics) sIn.(kOb) sIn.(bOb)
+  | Encrypt _ => mkState sIn.(keys) sIn.(basics)
+                                       ((obligationsK m) ++ sIn.(kOb))
+                                       ((obligations m) ++ sIn.(bOb))                                                                    
+  | _ =>  sIn
+  end.
